\documentclass{article}
\usepackage{amsmath}
\usepackage[landscape,letterpaper]{geometry}
\begin{document}

\begin{align}
  \dot{x}\left(t\right) &= v\left(t\right)\cos\left(\theta\left(t\right)\right)\\
  \dot{y}\left(t\right) &= v\left(t\right)\sin\left(\theta\left(t\right)\right)\\
  \dot{\theta}\left(t\right) &= \frac{\tan \phi\left(t\right)}{L} = \kappa\left(t\right)
\end{align}

\begin{align}
  \frac{\tan \phi\left(t\right)}{L} &= \kappa\left(t\right)\\
  \kappa_{\max} &= \frac{\tan \phi_{\max}}{L}
\end{align}

\begin{align}
  \kappa\left(t\right) = \left\{
    \begin{array}{cc}
      \kappa_{0}\left(t\right),   & t \le m/2\\
      \kappa_{1}\left(t\right), & m/2 < t\\
    \end{array}
  \right.
\end{align}

\begin{align}
  \kappa_{0}\left(t\right) &= \kappa_{\max}\frac{t}{\frac{m}{2}} &= &=2\kappa_{\max}\frac{t}{m}\\
  \kappa_{1}\left(t\right) &= \kappa_{\max}\left(1-\frac{t-\frac{m}{2}}{\frac{m}{2}}\right) &= \kappa_{\max}\left(1-\frac{2t-m}{m}\right) &= -2\kappa_{\max}\left(\frac{t}{m}-1\right)\end{align}

\begin{align}
  \theta\left(t\right) &= \int_0^t \dot{\theta}\left(x\right)\,dx = \int_0^t \kappa\left(x\right)\,dx\\
  &= \left\{
    \begin{array}{cc}
      \int_0^t \kappa_{0}\left(x\right)\,dx,   & t \le m/2\\
      \int_0^{m/2} \kappa_{0}\left(x\right)\,dx + \int_{m/2}^t \kappa_{1}\left(x\right)\,dx, & m/2 < t \le m\\
      \int_0^{m/2} \kappa_{0}\left(x\right)\,dx + \int_{m/2}^m \kappa_{1}\left(x\right)\,dx, & m < t
    \end{array}
  \right.
\end{align}

\begin{align}
  \int \kappa_{0}\left(x\right)\,dx &= \int 2\kappa_{\max}\frac{x}{m}\,dx &= \kappa_{\max}\frac{x^{2}}{m} + C_{0}\\
  \int \kappa_{1}\left(x\right)\,dx &= \int -2\kappa_{\max}\left(\frac{x}{m}-1\right)\,dx &= -\kappa_{\max}\left(\frac{x^{2}}{m}-2x\right) + C_{1}
\end{align}

\begin{align}
  \int_{0}^{t} \kappa_{0}\left(x\right)\,dx &= \kappa_{\max}\frac{t^{2}}{m}\\
  \int_{0}^{m/2} \kappa_{0}\left(x\right)\,dx &= \kappa_{\max}\frac{m}{4}
\end{align}

\begin{align}
  \int_{m/2}^{t} \kappa_{1}\left(x\right)\,dx &= -\kappa_{\max}\left(\frac{t^{2}}{m}-2t\right) + \kappa_{\max}\left(\frac{m}{4}-m\right) &= -\kappa_{\max}\left(\frac{t^{2}}{m}-2t\right) - \kappa_{\max}\frac{3m}{4}\\
  \int_{m/2}^{m} \kappa_{1}\left(x\right)\,dx &= -\kappa_{\max}\left(m-2m\right) + \kappa_{\max}\left(\frac{m}{4}-m\right) &= \kappa_{\max}\frac{m}{4}
\end{align}

\begin{align}
  \theta\left(t\right) &= \left\{
    \begin{array}{cc}
      \kappa_{\max} t^2 / m,   & t \le m/2\\
      -\kappa_{\max}\left(t^{2}/m-2t + m/2\right),& m/2 < t \le m\\
      \kappa_{\max}m/2, & m < t
    \end{array}
  \right.
\end{align}

\begin{align}
  x\left(t\right) &= \int_{0}^{t} \dot{x}\left(u\right)\,du\\
  &= \int_{0}^{t} v\left(u\right)\cos\left(\theta\left(u\right)\right)\,du\\
  &= v \int_{0}^{t} \cos\left(\theta\left(u\right)\right)\,du\\
  x\left(m\right) &= v \left(\int_{0}^{m/2} \cos\left(\frac{\kappa_{\max}}{m} u^2\right)\,du\right.\\
  &+ \left.\int_{m/2}^{m} \cos\left(-\kappa_{\max}\left(\frac{u^{2}}{m}-2u + \frac{m}{2}\right)\right)\,du\right)
\end{align}

\begin{align}
  y\left(t\right) &= \int_{0}^{t} \dot{y}\left(u\right)\,du\\
  &= \int_{0}^{t} v\left(u\right)\sin\left(\theta\left(u\right)\right)\,du\\
  &= v \int_{0}^{t} \sin\left(\theta\left(u\right)\right)\,du\\
  y\left(m\right) &= v \left(\int_{0}^{m/2} \sin\left(\frac{\kappa_{\max}}{m} u^2\right)\,du\right.\\
  &+ \left.\int_{m/2}^{m} \sin\left(-\kappa_{\max}\left(\frac{u^{2}}{m}-2u + \frac{m}{2}\right)\right)\,du\right)
\end{align}

\end{document}

%%% Local Variables:
%%% mode: latex
%%% TeX-master: t
%%% End:
